theories/RTL/Optimisation/RemoveNop.v
@@ -2,7 +2,7 @@ From RSL Require Import Prelude.
 
 From RSL.Logic Require Import Logic.
 From RSL.RTL Require Import SimRules.
-From RSL.Playground Require Import Identity.
+From RSL.RTL.Optimisation Require Import Commons.
 
 Import RTLNotations.
 
@@ -11,13 +11,6 @@ Definition is_nop (c : rtl_code) (pc: node) : option node :=
   | Some (Inop next) => Some next
   | _ => None
   end.
-
-Lemma is_nop_Some f pc pc':
-  is_nop (rtl_fn_code f) pc = Some pc' ->
-  f @ pc is <<{ nop -> pc' }>>.
-Proof using Type.
-  unfold is_nop. intros H. repeat case_match; congruence.
-Qed.
 
 Fixpoint find_next_pc (fuel: nat) (c: rtl_code) (n: node) : node :=
   match fuel with
@@ -28,17 +21,6 @@ Fixpoint find_next_pc (fuel: nat) (c: rtl_code) (n: node) : node :=
       | None => n
       end
   end.
-
-Lemma find_next_pc_O c n : find_next_pc 0 c n = n.
-Proof. done. Qed.
-
-Lemma find_next_pc_no_nop c n d :
-  is_nop c n = None -> find_next_pc d c n = n.
-Proof. destruct d; simpl; auto. by intros ->. Qed.
-
-Lemma find_next_pc_nop c n n' d' :
-  is_nop c n = Some n' -> find_next_pc (S d') c n = find_next_pc d' c n'.
-Proof. intros H. simpl. by rewrite H. Qed.
 
 Definition redirect_instr (f: node -> node) (i: rtl_instr) : rtl_instr :=
   match i with
@@ -53,9 +35,6 @@ Definition redirect_instr (f: node -> node) (i: rtl_instr) : rtl_instr :=
   | Ireturn reg => Ireturn reg
   end.
 
-Lemma redirect_instr_id i : redirect_instr (fun x => x) i = i.
-Proof using Type. by destruct i. Qed.
-
 Definition remove_nop_fun (depth: nat) (fn: rtl_function) : rtl_function :=
   let c := rtl_fn_code fn in
   let new_c := redirect_instr (find_next_pc depth c) <$> c in
@@ -68,77 +47,45 @@ Definition remove_nop_fun (depth: nat) (fn: rtl_function) : rtl_function :=
     rtl_fn_regs_no_dup := rtl_fn_regs_no_dup fn;
   |}.
 
-Lemma remove_nop_fun_equiv f : fun_equivalent (remove_nop_fun 0 f) f.
+Lemma remove_nop_ni {d} : name_identical (remove_nop_fun d).
+Proof using Type. by intros []. Qed.
+
+Lemma is_nop_Some f pc pc':
+  is_nop (rtl_fn_code f) pc = Some pc' ->
+  f @ pc is <<{ nop -> pc' }>>.
 Proof using Type.
-  destruct f as [fn regs ? c ?]. split_and!; simpl; auto.
-  apply map_eq. intros pc. rewrite lookup_fmap.
-  destruct (c !! pc) as [i | ] eqn:He; rewrite He; auto.
-  simpl. f_equal. apply redirect_instr_id.
+  unfold is_nop. intros H. repeat case_match; congruence.
 Qed.
 
-Lemma remove_nop_fun_no_dup {Ps} d:
-  is_no_dup (rtl_fn_name <$> prog_fun_list Ps) = true ->
-  is_no_dup (rtl_fn_name <$> fmap (remove_nop_fun d) (prog_fun_list Ps)) = true.
-Proof using Type.
-  rewrite !is_no_dup_sound.
-  induction (prog_fun_list Ps) as [ | f l IH ].
-  - done.
-  - simpl. intros H. inv H as [| ? ? HnIn HnDup].
-    constructor; auto.
-    intros (? & Heq & (f' & -> & H)%list_elem_of_fmap)%list_elem_of_fmap.
-    apply HnIn. rewrite Heq.
-    apply list_elem_of_fmap.
-    by exists f'.
-Qed.
+Lemma find_next_pc_O c n : find_next_pc 0 c n = n.
+Proof. done. Qed.
 
-Lemma remove_nop_fun_list {Ps} d fn f:
-  find_fun_in_list (prog_fun_list Ps) fn = Some f ->
-  find_fun_in_list (remove_nop_fun d <$> prog_fun_list Ps) fn = Some (remove_nop_fun d f).
-Proof using Type.
-  unfold find_fun_in_list.
-  intros ([? f'] & H & Heq)%fmap_Some. simpl in Heq. subst f'.
-  apply list_find_Some in H as (Hres & Hp & Hfirst).
-  rewrite fmap_Some. eexists (_, _). split; last reflexivity.
-  apply list_find_Some. split_and!.
-  - apply list_lookup_fmap_Some. by eexists.
-  - done.
-  - intros j ? (f' & -> & Hin)%list_lookup_fmap_Some Hj. simpl.
-    by eapply Hfirst.
-Qed.
+Lemma find_next_pc_no_nop c n d :
+  is_nop c n = None -> find_next_pc d c n = n.
+Proof. destruct d; simpl; auto. by intros ->. Qed.
 
-Lemma remove_nop_fun_main_some {Ps} d:
-  is_Some (find_fun_in_list (prog_fun_list Ps) (prog_main Ps)) ->
-  is_Some (find_fun_in_list (remove_nop_fun d <$> prog_fun_list Ps) (prog_main Ps)).
-Proof using Type. intros [f H]. eexists. by apply remove_nop_fun_list. Qed.
+Lemma find_next_pc_nop c n n' d' :
+  is_nop c n = Some n' -> find_next_pc (S d') c n = find_next_pc d' c n'.
+Proof. intros H. simpl. by rewrite H. Qed.
 
 Definition remove_nop (depth: nat) (p: rtl_program) : rtl_program :=
   {|
     prog_fun_list := remove_nop_fun depth <$> prog_fun_list p;
     prog_main := prog_main p;
-    prog_fun_list_no_dup := remove_nop_fun_no_dup depth (prog_fun_list_no_dup p);
-    prog_main_exists := remove_nop_fun_main_some depth (prog_main_exists p)
+    prog_fun_list_no_dup := opt_no_dup remove_nop_ni (prog_fun_list_no_dup p);
+    prog_main_exists := opt_main_some remove_nop_ni (prog_main_exists p)
   |}.
 
 Lemma remove_nop_find_fun {Ps} d fn f:
   find_fun Ps fn = Some f ->
   find_fun (remove_nop d Ps) fn = Some (remove_nop_fun d f).
-Proof using Type. by apply remove_nop_fun_list. Qed.
+Proof using Type. by apply opt_fun_list. Qed.
 
-Lemma remove_nop_incl p fn fs :
-  find_fun p fn = Some fs ->
-  ∃ ft, find_fun (remove_nop 0 p) fn = Some ft ∧ fun_equivalent ft fs.
-Proof using Type.
-  intros H. eexists.
-  split.
-  - by apply remove_nop_find_fun.
-  - by apply remove_nop_fun_equiv.
-Qed.
-
-Section no_opt.
+Section remove_nop.
   Context (Ps : prog rtl_lang) (depth : nat).
   Let Pt : prog rtl_lang := remove_nop depth Ps.
 
-  Definition no_opt_sim_inv : SInv rtl_lang rtl_lang WfNat WfNat :=
+  Definition remove_nop_sim_inv : SInv rtl_lang rtl_lang WfNat WfNat :=
     fun st j i ss ϕ =>
       (∃ I f d pct pcs ρt ρs,
           ⌜st = ([], State (remove_nop_fun depth f) pct ρt)⌟ ∗
@@ -149,14 +96,14 @@ Section no_opt.
           (∀ vt vs, samer I vt vs -∗ ϕ vt vs)
       )%I.
 
-  Lemma no_opt_soundness C f I :
+  Lemma remove_nop_soundness C f I :
     ⊢ [Pt, Ps, C] {{ same_args I }} (remove_nop_fun depth f) <{0, 0}= f {{ samer I }}.
   Proof using Type.
     iIntros "!>" (valt vals Ψ) "[%Harg Hinj] Hpost".
     iApply (source_callstate_exploit).
     iIntros (ρs pc Hlen -> ->).
     iApply (target_callstate); auto; first by eapply Forall2_length_r.
-    iApply (coind (no_opt_sim_inv)).
+    iApply (coind (remove_nop_sim_inv)).
     {
       clear.
       iIntros "!>" (C st j i ss ϕ) "#CIH".
@@ -178,8 +125,7 @@ Section no_opt.
             ]
           |] eqn:Hi.
 
-        - (* Inop is now a genuine, synced case, not exfalso *)
-          iApply (source_nop); first done.
+        - iApply (source_nop); first done.
           iApply (target_nop). { simpl. rewrite lookup_fmap Hi. by simpl. }
           iApply "CIH"; try (iPureIntro; simpl; lia).
           iExists I, f, depth, _, _, _, _. iFrame. iPureIntro. by split_and!.
@@ -305,11 +251,12 @@ Section no_opt.
             | r tpc fpc
             | r
             ]
-          |] eqn:Hi.
+          |] eqn:Hs;
+          try (eassert (Ht: remove_nop_fun depth f @ pcs is _);
+           [simpl; rewrite lookup_fmap Hs; by simpl|]).
 
-        - (* Inop is now a genuine, synced case, not exfalso *)
-          iApply (source_nop); first done.
-          iApply (target_nop). { simpl. rewrite lookup_fmap Hi. by simpl. }
+        - iApply (source_nop); first done.
+          iApply (target_nop); first done.
           iApply "CIH"; try (iPureIntro; simpl; lia).
           iExists I, f, depth, _, _, _, _. iFrame. iPureIntro. by split_and!.
 
@@ -317,15 +264,13 @@ Section no_opt.
           iApply (source_op_exploit); try done.
           iIntros (vs Hvs).
           destruct (eval_op_same_args Hval Hvs) as (vt & Hvt & Hrel).
-          iApply (target_op).
-          { simpl. rewrite lookup_fmap Hi. by simpl. } all: try done.
+          iApply (target_op); try done.
           iApply "CIH"; simpl; try (iPureIntro; lia).
           iExists I, f, _, _, _, _, _. iFrame. iPureIntro.
           split_and!; try done. by apply update_same_bank.
 
-        - destruct (Hsame src) as (vt & vs & Ht & Hs & Hv).
-          iApply (both_load with "[Hpost] Hinj").
-          { simpl. rewrite lookup_fmap Hi. by simpl. } all: try done.
+        - destruct (Hsame src) as (vt & vs & Hvt & Hvs & Hv).
+          iApply (both_load with "[Hpost] Hinj"); try done.
           iIntros (vt' vs' Hv') "Hinj".
           iApply "CIH"; try (iPureIntro; simpl; lia).
           iExists I, f, _, _, _, _, _. iFrame. iPureIntro. split_and!; try done.
@@ -333,14 +278,12 @@ Section no_opt.
 
         - destruct (Hsame src) as (addrt & addrs & Haddrt & Haddrs & Haddr).
           destruct (Hsame dst) as (dstt & dsts & Hdstt & Hdsts & Hdst).
-          iApply (both_store with "[Hpost] Hinj").
-          { simpl. rewrite lookup_fmap Hi. by simpl. } all: try done.
+          iApply (both_store with "[Hpost] Hinj"); try done.
           iIntros "Hinj".
           iApply "CIH"; try (iPureIntro; simpl; lia).
           iExists I, f, _, _, _, _, _. iFrame. iPureIntro. by split_and!.
 
-        - iApply (both_alloc with "[Hpost] Hinj").
-          { simpl. rewrite lookup_fmap Hi. by simpl. } all: try done.
+        - iApply (both_alloc with "[Hpost] Hinj"); try done.
           iIntros (lt ls vt vs Hrel) "Ht Hs Hinj".
           iApply "CIH"; try (iPureIntro; simpl; lia).
           iPoseProof (inj_insert_points_to with "Hinj Ht Hs [//]") as "H"; eauto.
@@ -358,16 +301,15 @@ Section no_opt.
             iApply (samer_mono with "Hsame"). by set_solver.
 
         - destruct (Hsame src) as (addrt & addrs & Haddrt & Haddrs & Haddr).
-          iApply (both_free with "[Hpost] Hinj").
-          { simpl. rewrite lookup_fmap Hi. by simpl. } all: try done.
+          iApply (both_free with "[Hpost] Hinj"); try done.
           iIntros "Hinj".
           iApply "CIH"; try (iPureIntro; simpl; lia).
           iExists I, f, _, _, _, _, _. iFrame. iPureIntro. by split_and!.
 
         - destruct (find_fun Ps fname) as [fn |] eqn:Hfn; last by iApply (source_call_fail).
           destruct (multiple_same args Hsame) as (vals & valt & Hvalt & Hvals & Hval).
-          iApply (both_call_framed (same_args I) (samer I) with "[] [Hinj] Hpost").
-          { simpl. rewrite lookup_fmap Hi. by simpl. } all: eauto.
+          iApply (both_call_framed (same_args I) (samer I) with "[] [Hinj] Hpost");
+            try done.
           + by apply remove_nop_find_fun.
           + clear.
             iIntros "!>" (valt vals Ψ) "[%Harg Hinj] Hpost".
@@ -394,16 +336,14 @@ Section no_opt.
         - destruct (Hsame r) as (bt & bs & Hbt & Hbs & Hb).
           iApply (source_if_exploit); try done.
           iIntros (b pc' -> ->). inv Hb.
-          iApply (target_if).
-          { simpl. rewrite lookup_fmap Hi. by simpl. } all: try done.
+          iApply (target_if); try done.
           iApply "CIH"; try (iPureIntro; simpl; lia).
           iExists I, f, _, _, _, _, _. iFrame. iPureIntro.
           split_and!; try done. by destruct b.
 
         - destruct (Hsame r) as (vt & vs & Hvt & Hvs & Hr).
           iApply (source_ret); try done.
-          iApply (target_ret).
-          { simpl. rewrite lookup_fmap Hi. by simpl. } all: try done.
+          iApply (target_ret); try done.
           iApply (both_ret). iApply "Hpost".
           iExists I. iFrame. by iPureIntro.
 
@@ -413,4 +353,4 @@ Section no_opt.
     iExists _, _, _, _, _, _, _. iFrame. iPureIntro.
     split_and!; try done. by apply init_same_bank.
   Qed.
-End no_opt.
+End remove_nop.
