theories/RTL/Optimisation/Commons.v
@@ -1,0 +1,40 @@
+From RSL Require Import Prelude.
+
+From RSL.RTL Require Import RTL.
+
+Definition name_identical o : Prop := ∀ f, rtl_fn_name f = rtl_fn_name (o f).
+
+Lemma opt_no_dup {Ps o} (Ho: name_identical o):
+  is_no_dup (rtl_fn_name <$> prog_fun_list Ps) = true ->
+  is_no_dup (rtl_fn_name <$> fmap o (prog_fun_list Ps)) = true.
+Proof using Type.
+  rewrite !is_no_dup_sound.
+  induction (prog_fun_list Ps) as [ | f l IH ].
+  - done.
+  - simpl. intros H. inv H as [| ? ? HnIn HnDup].
+    constructor; auto.
+    intros (? & Heq & (f' & -> & H)%list_elem_of_fmap)%list_elem_of_fmap.
+    apply HnIn. rewrite Ho, Heq.
+    apply list_elem_of_fmap.
+    by exists f'.
+Qed.
+
+Lemma opt_fun_list {Ps o} (Ho: name_identical o) fn f:
+  find_fun_in_list (prog_fun_list Ps) fn = Some f ->
+  find_fun_in_list (o <$> prog_fun_list Ps) fn = Some (o f).
+Proof using Type.
+  unfold find_fun_in_list.
+  intros ([? f'] & H & Heq)%fmap_Some. simpl in Heq. subst f'.
+  apply list_find_Some in H as (Hres & Hp & Hfirst).
+  rewrite fmap_Some. eexists (_, _). split; last reflexivity.
+  apply list_find_Some. split_and!.
+  - apply list_lookup_fmap_Some. by eexists.
+  - by rewrite <-Ho.
+  - intros j ? (f' & -> & Hin)%list_lookup_fmap_Some Hj. simpl.
+    rewrite <-Ho. by eapply Hfirst.
+Qed.
+
+Lemma opt_main_some {Ps o} (Ho: name_identical o):
+  is_Some (find_fun_in_list (prog_fun_list Ps) (prog_main Ps)) ->
+  is_Some (find_fun_in_list (o <$> prog_fun_list Ps) (prog_main Ps)).
+Proof using Type. intros [f H]. eexists. by apply opt_fun_list. Qed.
