theories/RTL/Optimisation/Simple.v
@@ -1,0 +1,275 @@
+From RSL Require Import Prelude.
+
+From RSL.Logic Require Import Logic.
+From RSL.RTL Require Import SimRules.
+From RSL.RTL.Optimisation Require Import Commons.
+
+Import RTLNotations.
+
+Definition simple_opt_instr (i: rtl_instr) : rtl_instr :=
+  match i with
+  | Iop op args dst pc =>
+      match op, args with
+      | Sub, [src1; src2] =>
+          if (src1 =? src2)
+          then Iop (ImmInt 0%Z) [] dst pc
+          else i
+      | Move, [src] =>
+          if (src =? dst)
+          then Inop pc
+          else i
+      | _, _ => i
+      end
+  | Icond b pcT pcF =>
+      if (pcT  =? pcF)
+      then Inop pcT
+      else Icond b pcT pcF
+  | _ => i
+  end.
+
+Definition simple_opt_fun (fn: rtl_function) : rtl_function :=
+  {|
+    rtl_fn_name := rtl_fn_name fn;
+    rtl_fn_regs := rtl_fn_regs fn;
+    rtl_fn_entrypoint := rtl_fn_entrypoint fn;
+    rtl_fn_code := simple_opt_instr <$> rtl_fn_code fn;
+    rtl_fn_regs_no_dup := rtl_fn_regs_no_dup fn;
+  |}.
+
+Lemma simple_opt_ni : name_identical simple_opt_fun.
+Proof using Type. by intros []. Qed.
+
+Definition simple_opt (p: rtl_program) : rtl_program :=
+  {|
+    prog_fun_list := simple_opt_fun <$> prog_fun_list p;
+    prog_main := prog_main p;
+    prog_fun_list_no_dup := opt_no_dup simple_opt_ni (prog_fun_list_no_dup p);
+    prog_main_exists := opt_main_some simple_opt_ni (prog_main_exists p)
+  |}.
+
+Lemma simple_opt_instr_case op args dst pc :
+  (
+    op = Move ∧
+    args = [dst] ∧
+    simple_opt_instr (Iop op args dst pc) = Inop pc
+  ) ∨ (
+    ∃ src,
+      op = Sub ∧
+      args = [src; src] ∧
+      simple_opt_instr (Iop op args dst pc) = Iop (ImmInt 0%Z) [] dst pc
+  ) ∨ (
+    simple_opt_instr (Iop op args dst pc) = Iop op args dst pc
+  ).
+Proof using Type.
+  destruct op, args as [|src1 [|src2 []]]; try (by do 2 right).
+  - destruct (src1 =? src2) eqn:Heq.
+    + right. left. eexists. split_and!; auto.
+      * by apply Nat.eqb_eq in Heq as ->.
+      * simpl. by rewrite Heq.
+    + do 2 right. simpl. by rewrite Heq.
+  - destruct (src1 =? dst) eqn:Heq.
+    + left. split_and!; auto.
+      * by apply Nat.eqb_eq in Heq as ->.
+      * simpl. by rewrite Heq.
+    + do 2 right. simpl. by rewrite Heq.
+Qed.
+
+Lemma simple_opt_find_fun {Ps} fn f:
+  find_fun Ps fn = Some f ->
+  find_fun (simple_opt Ps) fn = Some (simple_opt_fun f).
+Proof using Type. by apply opt_fun_list. Qed.
+
+Section simple_opt.
+  Context (Ps : prog rtl_lang).
+  Let Pt : prog rtl_lang := simple_opt Ps.
+
+  Definition simple_opt_sim_inv : SInv rtl_lang rtl_lang WfNat WfNat :=
+    fun st j i ss ϕ =>
+      (∃ I f pc ρt ρs,
+          ⌜st = ([], State (simple_opt_fun f) pc ρt)⌟ ∗
+          ⌜ss = ([], State f pc ρs)⌟ ∗
+          ⌜∀ r, ρt@r <{ I }> ρs@r⌟ ∗
+          mem_inj I ∅ ∗
+          (∀ vt vs, samer I vt vs -∗ ϕ vt vs)
+      )%I.
+
+  Lemma simple_opt_soundness C f I :
+    ⊢ [Pt, Ps, C] {{ same_args I }} (simple_opt_fun f) <{0, 0}= f {{ samer I }}.
+  Proof using Type.
+    iIntros "!>" (valt vals Ψ) "[%Harg Hinj] Hpost".
+    iApply (source_callstate_exploit).
+    iIntros (ρs pc Hlen -> ->).
+    iApply (target_callstate); auto; first by eapply Forall2_length_r.
+    iApply (coind (simple_opt_sim_inv)).
+    {
+      clear.
+      iIntros "!>" (C st j i ss ϕ) "#CIH".
+      iIntros "(%I & %f & %pc & %ρt & %ρs & -> & -> & %Hsame & Hinj & Hpost)".
+
+      destruct ((rtl_fn_code f) !! pc)
+        as [
+          [ pc'
+          | op args dst pc'
+          | src dst pc'
+          | dst src pc'
+          | dst pc'
+          | src pc'
+          | fname args dst pc'
+          | r tpc fpc
+          | r
+          ]
+        |] eqn:Hi.
+
+      - iApply (source_nop); first done.
+        iApply (target_nop). { simpl. rewrite lookup_fmap Hi. by simpl. }
+        iApply "CIH"; try (iPureIntro; simpl; lia).
+        iExists I, f, _, _, _. iFrame. iPureIntro. by split_and!.
+
+      - destruct (multiple_same args Hsame) as (valt & vals & Hvalt & Hvals & Hval).
+        iApply (source_op_exploit); try done.
+        iIntros (vs Hvs).
+        destruct (simple_opt_instr_case op args dst pc') as
+          [ (-> & -> & H) | [(? & -> & -> & H) | H]].
+
+        + iApply (target_nop).
+          { simpl. rewrite lookup_fmap Hi. eapply fmap_Some.
+            eexists. split; [ done | by rewrite H ]. }
+
+          assert (∃ v, vals = [v]) as (v & ->).
+          { pose proof (regbank_list_length _ _ _ Hvals) as Hlen.
+            destruct vals as [|? [|]]; try inv Hlen. by eexists. }
+          inv Hval as [ | ? ? ? ? ? Hforall ]; inv Hforall.
+          apply regbank_assert_unfold in Hvals as [Hval _]. inv Hvs.
+
+          iApply "CIH"; simpl; try (iPureIntro; lia).
+          iExists I, f, _, _, _. iFrame. iPureIntro.
+          split_and!; try done. by apply same_bank_set_useless.
+
+        + iApply (target_op).
+          { simpl. rewrite lookup_fmap Hi. eapply fmap_Some.
+            eexists. split; [ done | by rewrite H ]. } all: try done.
+
+          assert (∃ v, vals = [v; v]) as (v & ->).
+          { pose proof (regbank_list_length _ _ _ Hvals) as Hlen.
+            destruct vals as [|? [|? []]]; try inv Hlen.
+            apply regbank_assert_unfold in Hvals as [? Hvals].
+            apply regbank_assert_unfold in Hvals as [? _]. simregs.
+            by eexists. }
+          inv Hval as [ | ? ? ? ? ? Hforall ];
+            inv Hforall  as [ | ? ? ? ? ? Hforall' ]; inv Hforall'.
+          destruct v as [vi | | | ]; inv Hvs.
+          rewrite Z.sub_diag.
+
+          iApply "CIH"; simpl; try (iPureIntro; lia).
+          iExists I, f, _, _, _. iFrame. iPureIntro.
+          split_and!; try done. apply update_same_bank.
+          * by constructor.
+          * done.
+
+        + destruct (eval_op_same_args Hval Hvs) as (vt & Hvt & Hrel).
+          iApply (target_op).
+          { simpl. rewrite lookup_fmap Hi. eapply fmap_Some.
+            eexists. split; [ done | by rewrite H ]. } all: try done.
+
+          iApply "CIH"; simpl; try (iPureIntro; lia).
+          iExists I, f, _, _, _. iFrame. iPureIntro.
+          split_and!; try done. by apply update_same_bank.
+
+
+      - destruct (Hsame src) as (vt & vs & Ht & Hs & Hv).
+        iApply (both_load with "[Hpost] Hinj").
+        { simpl. rewrite lookup_fmap Hi. by simpl. } all: try done.
+        iIntros (vt' vs' Hv') "Hinj".
+        iApply "CIH"; try (iPureIntro; simpl; lia).
+        iExists I, f, _, _, _. iFrame. iPureIntro. split_and!; try done.
+        by apply update_same_bank.
+
+      - destruct (Hsame src) as (addrt & addrs & Haddrt & Haddrs & Haddr).
+        destruct (Hsame dst) as (dstt & dsts & Hdstt & Hdsts & Hdst).
+        iApply (both_store with "[Hpost] Hinj").
+        { simpl. rewrite lookup_fmap Hi. by simpl. } all: try done.
+        iIntros "Hinj".
+        iApply "CIH"; try (iPureIntro; simpl; lia).
+        iExists I, f, _, _, _. iFrame. iPureIntro. by split_and!.
+
+      - iApply (both_alloc with "[Hpost] Hinj").
+        { simpl. rewrite lookup_fmap Hi. by simpl. } all: try done.
+        iIntros (lt ls vt vs Hrel) "Ht Hs Hinj".
+        iApply "CIH"; try (iPureIntro; simpl; lia).
+        iPoseProof (inj_insert_points_to with "Hinj Ht Hs [//]") as "H"; eauto.
+        iExists _, f, _, _, _. iFrame.
+        iSplitR. { by iPureIntro. }
+        iSplitR. { by iPureIntro. }
+        iSplitR.
+        + iPureIntro. apply update_same_bank.
+          * constructor. unfold related. by set_solver.
+          * intros ? _. eapply same_bank_mono; last done. by set_solver.
+        + clear.
+          iIntros (vt vs) "Hsame".
+          iApply "Hpost".
+          iApply (samer_mono with "Hsame"). by set_solver.
+
+      - destruct (Hsame src) as (addrt & addrs & Haddrt & Haddrs & Haddr).
+        iApply (both_free with "[Hpost] Hinj").
+        { simpl. rewrite lookup_fmap Hi. by simpl. } all: try done.
+        iIntros "Hinj".
+        iApply "CIH"; try (iPureIntro; simpl; lia).
+        iExists I, f, _, _, _. iFrame. iPureIntro. by split_and!.
+
+      - destruct (find_fun Ps fname) as [fn |] eqn:Hfn; last by iApply (source_call_fail).
+        destruct (multiple_same args Hsame) as (vals & valt & Hvalt & Hvals & Hval).
+        iApply (both_call_framed (same_args I) (samer I) with "[] [Hinj] Hpost").
+        { simpl. rewrite lookup_fmap Hi. by simpl. } all: eauto.
+        + by apply simple_opt_find_fun.
+        + clear.
+          iIntros "!>" (valt vals Ψ) "[%Harg Hinj] Hpost".
+          iApply (source_callstate_exploit).
+          iIntros (ρs pc Hlen -> ->).
+          iApply (target_callstate); auto; first by eapply Forall2_length_r.
+          iApply "CIH"; simpl; try (iPureIntro; lia).
+          iExists I, fn, _, _, _.  iFrame. iPureIntro.
+          split_and!; try done. by apply init_same_bank.
+
+        + iFrame. by iPureIntro.
+
+        + iIntros "!>" (j' i' ? ? ? ?) "(%I' & %Hincl & %Hsame' & Hinj) Hpost".
+          iApply "CIH"; auto.
+          iExists I', f, _, _, _. iFrame.
+          iSplitR. { by iPureIntro. }
+          iSplitR. { by iPureIntro. }
+          iSplitR.
+          * iPureIntro. apply update_same_bank; first done.
+            intros ? ?. by eapply same_bank_mono, Hsame.
+          * iIntros (? ?) "Hsame". iApply "Hpost". by iApply (samer_mono with "Hsame").
+
+      - destruct (Hsame r) as (bt & bs & Hbt & Hbs & Hb).
+        iApply (source_if_exploit); try done.
+        iIntros (b pc' -> ->). inv Hb.
+        destruct (decide (tpc = fpc)) as [-> | Hneq].
+        + iApply (target_nop).
+          { simpl. rewrite lookup_fmap Hi. simpl. by rewrite Nat.eqb_refl. }
+          iApply "CIH"; simpl; try (iPureIntro; lia).
+          iExists I, f, _, _, _.  iFrame. iPureIntro.
+          split_and!; try done. by destruct b.
+        + apply Nat.eqb_neq in Hneq.
+          iApply (target_if).
+          { simpl. rewrite lookup_fmap Hi. simpl. by rewrite Hneq. }
+          all: try done.
+          iApply "CIH"; simpl; try (iPureIntro; lia).
+          iExists I, f, _, _, _.  iFrame. iPureIntro.
+          by split_and!.
+
+      - destruct (Hsame r) as (vt & vs & Hvt & Hvs & Hr).
+        iApply (source_ret); try done.
+        iApply (target_ret).
+        { simpl. rewrite lookup_fmap Hi. by simpl. } all: try done.
+        iApply (both_ret). iApply "Hpost".
+        iExists I. iFrame. by iPureIntro.
+
+      - by iApply (source_fail).
+
+    }
+    iExists _, _, _, _, _. iFrame. iPureIntro.
+    split_and!; try done. by apply init_same_bank.
+  Qed.
+End simple_opt.
